extract lib, not main

src/mini_ledger/proofs/fstar/extraction/Mini_ledger.fst
@@ -2,35 +2,1533 @@ module Mini_ledger
 #set-options "--fuel 0 --ifuel 1 --z3rlimit 15"
 open Core
 
-let v___export_service: Alloc.String.t_String =
-  let service:Alloc.Vec.t_Vec (Alloc.String.t_String & Candid.Types.Internal.t_Type)
-    Alloc.Alloc.t_Global =
-    Alloc.Vec.new_under_impl
-  in
-  let env:Candid.Types.Internal.t_TypeContainer = Candid.Types.Internal.new_under_impl_3 in
-  let service:Alloc.Vec.t_Vec (Alloc.String.t_String & Candid.Types.Internal.t_Type)
-    Alloc.Alloc.t_Global =
-    Core.Slice.sort_unstable_by_key_under_impl service
-      (fun (name, _) -> Core.Clone.Clone.clone name <: Alloc.String.t_String)
-  in
-  let ty:Candid.Types.Internal.t_Type = Candid.Types.Internal.Type_Service service in
-  let actor:Core.Option.t_Option Candid.Types.Internal.t_Type = Core.Option.Option_Some ty in
-  let result:Alloc.String.t_String =
-    Candid.Bindings.Candid.compile env.Candid.Types.Internal.TypeContainer.f_env actor
-  in
-  Alloc.Fmt.format (Core.Fmt.new_v1_under_impl_2 (Rust_primitives.unsize (let list = [""] in
-              FStar.Pervasives.assert_norm (Prims.eq2 (List.Tot.length list) 1);
-              Rust_primitives.Hax.array_of_list list)
-          <:
-          slice string)
-        (Rust_primitives.unsize (let list =
-                [Core.Fmt.Rt.new_display_under_impl_1 result <: Core.Fmt.Rt.t_Argument]
-              in
-              FStar.Pervasives.assert_norm (Prims.eq2 (List.Tot.length list) 1);
-              Rust_primitives.Hax.array_of_list list)
-          <:
-          slice Core.Fmt.Rt.t_Argument)
-      <:
-      Core.Fmt.t_Arguments)
+let v_PERMITTED_DRIFT: Core.Time.t_Duration = Core.Time.from_secs_under_impl_1 60uL
 
-let main: Prims.unit = ()
+type t_TransferError =
+  | TransferError_BadFee { f_expected_fee:Mini_ledger_core.Tokens.t_Tokens }: t_TransferError
+  | TransferError_InsufficientFunds { f_balance:Mini_ledger_core.Tokens.t_Tokens }: t_TransferError
+  | TransferError_TxTooOld { f_allowed_window_nanos:u64 }: t_TransferError
+  | TransferError_TxCreatedInFuture { f_ledger_time:Mini_ledger_core.Timestamp.t_TimeStamp }: t_TransferError
+  | TransferError_TxThrottled : t_TransferError
+  | TransferError_TxDuplicate { f_duplicate_of:u64 }: t_TransferError
+
+let v___: Prims.unit = ()
+
+let v___1: Prims.unit = ()
+
+class t_LedgerTransaction (v_Self: Type) = {
+  accountId:Type;
+  accountId_implements_t_Eq:Core.Cmp.t_Eq _;
+  accountId_implements_t_PartialEq:Core.Cmp.t_PartialEq _ _;
+  accountId_implements_t_Hash:Core.Hash.t_Hash _;
+  accountId_implements_t_Sized:Core.Marker.t_Sized _;
+  burn:
+      _ ->
+      Mini_ledger_core.Tokens.t_Tokens ->
+      Core.Option.t_Option Mini_ledger_core.Timestamp.t_TimeStamp ->
+      Core.Option.t_Option u64
+    -> self;
+  created_at_time:self -> Core.Option.t_Option Mini_ledger_core.Timestamp.t_TimeStamp;
+  hash:self -> Mini_ledger_core.Block.t_HashOf self;
+  apply:self -> l -> (l & Core.Result.t_Result Prims.unit Mini_ledger_core.Balances.t_BalanceError)
+}
+
+let impl: t_LedgerTransaction Mini_ledger.Transaction.t_Transaction =
+  {
+    accountId = Mini_ledger.Account.t_Account;
+    burn
+    =
+    (fun
+        (from: Mini_ledger.Account.t_Account)
+        (amount: Mini_ledger_core.Tokens.t_Tokens)
+        (created_at_time: Core.Option.t_Option Mini_ledger_core.Timestamp.t_TimeStamp)
+        (memo: Core.Option.t_Option u64)
+        ->
+        {
+          Mini_ledger.Transaction.Transaction.f_operation
+          =
+          Mini_ledger.Transaction.Operation_Burn
+          ({
+              Mini_ledger.Transaction.Operation.Burn.f_from = from;
+              Mini_ledger.Transaction.Operation.Burn.f_amount
+              =
+              Mini_ledger_core.Tokens.get_e8s_under_impl amount
+            });
+          Mini_ledger.Transaction.Transaction.f_created_at_time
+          =
+          Core.Option.map_under_impl created_at_time
+            (fun t -> Mini_ledger_core.Timestamp.as_nanos_since_unix_epoch_under_impl t <: u64);
+          Mini_ledger.Transaction.Transaction.f_memo
+          =
+          Core.Option.map_under_impl memo Core.Convert.From.from
+        });
+    created_at_time
+    =
+    (fun (self: Mini_ledger.Transaction.t_Transaction) ->
+        Core.Option.map_under_impl self.Mini_ledger.Transaction.Transaction.f_created_at_time
+          Mini_ledger_core.Timestamp.from_nanos_since_unix_epoch_under_impl);
+    hash
+    =
+    (fun (self: Mini_ledger.Transaction.t_Transaction) ->
+        let cbor_bytes:Alloc.Vec.t_Vec u8 Alloc.Alloc.t_Global = Alloc.Vec.new_under_impl in
+        let tmp0, out:(Alloc.Vec.t_Vec u8 Alloc.Alloc.t_Global &
+          Core.Result.t_Result Prims.unit (Ciborium.Ser.Error.t_Error _)) =
+          Ciborium.Ser.into_writer self cbor_bytes
+        in
+        let cbor_bytes:Alloc.Vec.t_Vec u8 Alloc.Alloc.t_Global = tmp0 in
+        let hoist158:(Alloc.Vec.t_Vec u8 Alloc.Alloc.t_Global &
+          Core.Result.t_Result Prims.unit (Ciborium.Ser.Error.t_Error _)) =
+          out
+        in
+        let _:Prims.unit =
+          Core.Result.expect_under_impl hoist158 "bug: failed to encode a transaction"
+        in
+        Core.Result.unwrap_or_else_under_impl (Core.Result.map_under_impl (Mini_ledger.Hash.hash_cbor
+                  (Core.Ops.Deref.Deref.deref cbor_bytes <: slice u8)
+                <:
+                Core.Result.t_Result (array u8 32sz) Alloc.String.t_String)
+              Mini_ledger_core.Block.new_under_impl_2
+            <:
+            Core.Result.t_Result
+              (Mini_ledger_core.Block.t_HashOf Mini_ledger.Transaction.t_Transaction)
+              Alloc.String.t_String)
+          (fun err ->
+              Rust_primitives.Hax.never_to_any (Core.Panicking.panic_fmt (Core.Fmt.new_v1_under_impl_2
+                        (Rust_primitives.unsize (let list =
+                                ["bug: transaction CBOR "; " is not hashable: "]
+                              in
+                              FStar.Pervasives.assert_norm (Prims.eq2 (List.Tot.length list) 2);
+                              Rust_primitives.Hax.array_of_list list)
+                          <:
+                          slice string)
+                        (Rust_primitives.unsize (let list =
+                                [
+                                  Core.Fmt.Rt.new_display_under_impl_1 (Hex.encode cbor_bytes
+                                      <:
+                                      Alloc.String.t_String)
+                                  <:
+                                  Core.Fmt.Rt.t_Argument;
+                                  Core.Fmt.Rt.new_display_under_impl_1 err <: Core.Fmt.Rt.t_Argument
+                                ]
+                              in
+                              FStar.Pervasives.assert_norm (Prims.eq2 (List.Tot.length list) 2);
+                              Rust_primitives.Hax.array_of_list list)
+                          <:
+                          slice Core.Fmt.Rt.t_Argument)
+                      <:
+                      Core.Fmt.t_Arguments)
+                  <:
+                  Rust_primitives.Hax.t_Never)
+              <:
+              Mini_ledger_core.Block.t_HashOf Mini_ledger.Transaction.t_Transaction));
+    apply
+    =
+    fun (self: Mini_ledger.Transaction.t_Transaction) (ledger: l) ->
+      let ledger, output:(l &
+        (l & Core.Result.t_Result Prims.unit Mini_ledger_core.Balances.t_BalanceError)) =
+        match self.Mini_ledger.Transaction.Transaction.f_operation with
+        | Mini_ledger.Transaction.Operation_Transfer
+          { Mini_ledger.Transaction.Operation.Transfer.f_from = from ;
+            Mini_ledger.Transaction.Operation.Transfer.f_to = to ;
+            Mini_ledger.Transaction.Operation.Transfer.f_amount = amount ;
+            Mini_ledger.Transaction.Operation.Transfer.f_fee = fee } ->
+          let tmp0, out:(l &
+            Core.Result.t_Result Prims.unit Mini_ledger_core.Balances.t_BalanceError) =
+            Mini_ledger.LedgerData.transfer_balance ledger
+              from
+              to
+              (Mini_ledger_core.Tokens.from_e8s_under_impl amount
+                <:
+                Mini_ledger_core.Tokens.t_Tokens)
+              (Mini_ledger_core.Tokens.from_e8s_under_impl fee <: Mini_ledger_core.Tokens.t_Tokens)
+          in
+          let ledger:l = tmp0 in
+          ledger, out
+        | Mini_ledger.Transaction.Operation_Burn
+          { Mini_ledger.Transaction.Operation.Burn.f_from = from ;
+            Mini_ledger.Transaction.Operation.Burn.f_amount = amount } ->
+          let tmp0, out:(l &
+            Core.Result.t_Result Prims.unit Mini_ledger_core.Balances.t_BalanceError) =
+            Mini_ledger.LedgerData.burn_balance ledger
+              from
+              (Mini_ledger_core.Tokens.from_e8s_under_impl amount
+                <:
+                Mini_ledger_core.Tokens.t_Tokens)
+          in
+          let ledger:l = tmp0 in
+          ledger, out
+        | Mini_ledger.Transaction.Operation_Mint
+          { Mini_ledger.Transaction.Operation.Mint.f_to = to ;
+            Mini_ledger.Transaction.Operation.Mint.f_amount = amount } ->
+          let tmp0, out:(l &
+            Core.Result.t_Result Prims.unit Mini_ledger_core.Balances.t_BalanceError) =
+            Mini_ledger.LedgerData.mint_balance ledger
+              to
+              (Mini_ledger_core.Tokens.from_e8s_under_impl amount
+                <:
+                Mini_ledger_core.Tokens.t_Tokens)
+          in
+          let ledger:l = tmp0 in
+          ledger, out
+      in
+      ledger, output
+  }
+
+type t_Blockchain = {
+  f_blocks:Alloc.Vec.t_Vec Mini_ledger_core.Block.t_EncodedBlock Alloc.Alloc.t_Global;
+  f_last_hash:Core.Option.t_Option
+  (Mini_ledger_core.Block.t_HashOf Mini_ledger_core.Block.t_EncodedBlock);
+  f_last_timestamp:Mini_ledger_core.Timestamp.t_TimeStamp;
+  f_num_archived_blocks:u64
+}
+
+let v___2: Prims.unit = ()
+
+let v___3: Prims.unit = ()
+
+let impl: Core.Default.t_Default t_Blockchain =
+  {
+    default
+    =
+    fun  ->
+      {
+        Mini_ledger.Blockchain.f_blocks = Alloc.Vec.new_under_impl;
+        Mini_ledger.Blockchain.f_last_hash = Core.Option.Option_None;
+        Mini_ledger.Blockchain.f_last_timestamp
+        =
+        Mini_ledger_core.Timestamp.from_nanos_since_unix_epoch_under_impl 0uL;
+        Mini_ledger.Blockchain.f_num_archived_blocks = 0uL
+      }
+  }
+
+let chain_length_under_impl_2 (self: t_Blockchain) : u64 =
+  cast (Alloc.Vec.len_under_impl_1 self.Mini_ledger.Blockchain.f_blocks)
+
+let add_block_under_impl_2 (self: t_Blockchain) (block: b)
+    : (t_Blockchain & Core.Result.t_Result u64 Alloc.String.t_String) =
+  Rust_primitives.Hax.Control_flow_monad.Mexception.run (let* _:Prims.unit =
+        if
+          (Mini_ledger_core.Block.BlockType.parent_hash block
+            <:
+            Core.Option.t_Option
+            (Mini_ledger_core.Block.t_HashOf Mini_ledger_core.Block.t_EncodedBlock)) <>.
+          self.Mini_ledger.Blockchain.f_last_hash
+        then
+          let* hoist159:Rust_primitives.Hax.t_Never =
+            Core.Ops.Control_flow.ControlFlow.v_Break (self,
+                Core.Result.Result_Err
+                (Alloc.String.ToString.to_string "Cannot apply block because its parent hash doesn't match."
+
+                  <:
+                  Alloc.String.t_String))
+          in
+          Core.Ops.Control_flow.ControlFlow_Continue (Rust_primitives.Hax.never_to_any hoist159)
+        else Core.Ops.Control_flow.ControlFlow_Continue ()
+      in
+      let* _:Prims.unit =
+        if
+          (Mini_ledger_core.Block.BlockType.timestamp block
+            <:
+            Mini_ledger_core.Timestamp.t_TimeStamp) <.
+          self.Mini_ledger.Blockchain.f_last_timestamp
+        then
+          let* hoist160:Rust_primitives.Hax.t_Never =
+            Core.Ops.Control_flow.ControlFlow.v_Break (self,
+                Core.Result.Result_Err
+                (Alloc.Borrow.ToOwned.to_owned "Cannot apply block because its timestamp is older than the previous tip."
+
+                  <:
+                  _))
+          in
+          Core.Ops.Control_flow.ControlFlow_Continue (Rust_primitives.Hax.never_to_any hoist160)
+        else Core.Ops.Control_flow.ControlFlow_Continue ()
+      in
+      Core.Ops.Control_flow.ControlFlow_Continue
+      (let self:t_Blockchain =
+          {
+            self with
+            Mini_ledger.Blockchain.f_last_timestamp
+            =
+            Mini_ledger_core.Block.BlockType.timestamp block
+          }
+        in
+        let encoded_block:Mini_ledger_core.Block.t_EncodedBlock =
+          Mini_ledger_core.Block.BlockType.encode block
+        in
+        let self:t_Blockchain =
+          {
+            self with
+            Mini_ledger.Blockchain.f_last_hash
+            =
+            Core.Option.Option_Some (Mini_ledger_core.Block.BlockType.block_hash encoded_block)
+          }
+        in
+        let self:t_Blockchain =
+          {
+            self with
+            Mini_ledger.Blockchain.f_blocks
+            =
+            Alloc.Vec.push_under_impl_1 self.Mini_ledger.Blockchain.f_blocks encoded_block
+          }
+        in
+        let output:Core.Result.t_Result u64 Alloc.String.t_String =
+          Core.Result.Result_Ok
+          (Core.Option.unwrap_under_impl (Core.Num.checked_sub_under_impl_9 (chain_length_under_impl_2
+                      self
+                    <:
+                    u64)
+                  1uL
+                <:
+                Core.Option.t_Option u64))
+        in
+        self, output))
+
+let block_slice_under_impl_2 (self: t_Blockchain) (local_blocks: Core.Ops.Range.t_Range u64)
+    : slice Mini_ledger_core.Block.t_EncodedBlock =
+  self.Mini_ledger.Blockchain.f_blocks.[ {
+      Core.Ops.Range.Range.f_start = cast local_blocks.Core.Ops.Range.Range.f_start;
+      Core.Ops.Range.Range.f_end = cast local_blocks.Core.Ops.Range.Range.f_end
+    } ]
+
+class t_LedgerData (v_Self: Type) = {
+  accountId:Type;
+  accountId_implements_t_Clone:Core.Clone.t_Clone _;
+  accountId_implements_t_Eq:Core.Cmp.t_Eq _;
+  accountId_implements_t_PartialEq:Core.Cmp.t_PartialEq _ _;
+  accountId_implements_t_Ord:Core.Cmp.t_Ord _;
+  accountId_implements_t_PartialOrd:Core.Cmp.t_PartialOrd _ _;
+  accountId_implements_t_Hash:Core.Hash.t_Hash _;
+  accountId_implements_t_Sized:Core.Marker.t_Sized _;
+  block:Type;
+  block_implements_t_BlockType:Mini_ledger_core.Block.t_BlockType _;
+  block_implements_t_Sized:Core.Marker.t_Sized _;
+  transaction:Type;
+  transaction_implements_t_Clone:Core.Clone.t_Clone _;
+  transaction_implements_t_Ord:Core.Cmp.t_Ord _;
+  transaction_implements_t_PartialOrd:Core.Cmp.t_PartialOrd _ _;
+  transaction_implements_t_PartialEq:Core.Cmp.t_PartialEq _ _;
+  transaction_implements_t_Eq:Core.Cmp.t_Eq _;
+  transaction_implements_t_LedgerTransaction:t_LedgerTransaction _;
+  transaction_implements_t_Sized:Core.Marker.t_Sized _;
+  transaction_window:self -> Core.Time.t_Duration;
+  max_transactions_in_window:self -> usize;
+  max_transactions_to_purge:self -> usize;
+  max_number_of_accounts:self -> usize;
+  accounts_overflow_trim_quantity:self -> usize;
+  token_name:self -> string;
+  token_symbol:self -> string;
+  balances:self
+    -> Mini_ledger_core.Balances.t_Balances _
+        (Std.Collections.Hash.Map.t_HashMap _
+            Mini_ledger_core.Tokens.t_Tokens
+            Std.Collections.Hash.Map.t_RandomState);
+  transfer_balance:
+      self ->
+      Mini_ledger.Account.t_Account ->
+      Mini_ledger.Account.t_Account ->
+      Mini_ledger_core.Tokens.t_Tokens ->
+      Mini_ledger_core.Tokens.t_Tokens
+    -> (self & Core.Result.t_Result Prims.unit Mini_ledger_core.Balances.t_BalanceError);
+  mint_balance:self -> Mini_ledger.Account.t_Account -> Mini_ledger_core.Tokens.t_Tokens
+    -> (self & Core.Result.t_Result Prims.unit Mini_ledger_core.Balances.t_BalanceError);
+  burn_balance:self -> Mini_ledger.Account.t_Account -> Mini_ledger_core.Tokens.t_Tokens
+    -> (self & Core.Result.t_Result Prims.unit Mini_ledger_core.Balances.t_BalanceError);
+  blockchain:self -> t_Blockchain;
+  blockchain_add_block:self -> _ -> (self & Core.Result.t_Result u64 Alloc.String.t_String);
+  transactions_by_hash:self
+    -> Alloc.Collections.Btree.Map.t_BTreeMap (Mini_ledger_core.Block.t_HashOf _)
+        u64
+        Alloc.Alloc.t_Global;
+  remove_transactions_by_hash:self -> Mini_ledger_core.Block.t_HashOf _
+    -> (self & Core.Option.t_Option u64);
+  insert_transactions_by_hash:self -> Mini_ledger_core.Block.t_HashOf _ -> u64
+    -> (self & Core.Option.t_Option u64);
+  transactions_by_height:self
+    -> Alloc.Collections.Vec_deque.t_VecDeque (Mini_ledger.Transaction.t_TransactionInfo _)
+        Alloc.Alloc.t_Global;
+  pop_front_transactions_by_height:self -> self;
+  push_back_transactions_by_height:self -> Mini_ledger.Transaction.t_TransactionInfo _ -> self;
+  on_purged_transaction:self -> u64 -> self
+}
+
+let purge_old_transactions
+      (#l: Type)
+      (#[FStar.Tactics.Typeclasses.tcresolve ()] __0: Core.Marker.t_Sized l)
+      (#[FStar.Tactics.Typeclasses.tcresolve ()] __1: t_LedgerData l)
+      (ledger: l)
+      (now: Mini_ledger_core.Timestamp.t_TimeStamp)
+    : (l & usize) =
+  let max_tx_to_purge:usize = Mini_ledger.LedgerData.max_transactions_to_purge ledger in
+  let num_tx_purged_out:usize = 0sz in
+  let break_loop:bool = false in
+  let break_loop, ledger, num_tx_purged_out:(bool & l & usize) =
+    Core.Iter.Traits.Iterator.Iterator.fold (Core.Iter.Traits.Collect.IntoIterator.into_iter ({
+              Core.Ops.Range.Range.f_start = 0sz;
+              Core.Ops.Range.Range.f_end = max_tx_to_purge
+            })
+        <:
+        _)
+      (break_loop, ledger, num_tx_purged_out)
+      (fun (break_loop, ledger, num_tx_purged_out) num_tx_purged ->
+          if ~.break_loop <: bool
+          then
+            let num_tx_purged_out:usize = num_tx_purged in
+            match
+              Alloc.Collections.Vec_deque.front_under_impl_5 (Mini_ledger.LedgerData.transactions_by_height
+                    ledger
+                  <:
+                  Alloc.Collections.Vec_deque.t_VecDeque
+                    (Mini_ledger.Transaction.t_TransactionInfo _) Alloc.Alloc.t_Global)
+            with
+            | Core.Option.Option_Some tx_info ->
+              let break_loop:bool =
+                if
+                  ((tx_info.Mini_ledger.Transaction.TransactionInfo.f_block_timestamp +.
+                      (Mini_ledger.LedgerData.transaction_window ledger <: Core.Time.t_Duration)
+                      <:
+                      _) +.
+                    v_PERMITTED_DRIFT
+                    <:
+                    Mini_ledger_core.Timestamp.t_TimeStamp) >=.
+                  now
+                then
+                  let break_loop:bool = true in
+                  break_loop
+                else break_loop
+              in
+              let transaction_hash:Mini_ledger_core.Block.t_HashOf _ =
+                tx_info.Mini_ledger.Transaction.TransactionInfo.f_transaction_hash
+              in
+              let tmp0, out:(l & Core.Option.t_Option u64) =
+                Mini_ledger.LedgerData.remove_transactions_by_hash ledger transaction_hash
+              in
+              let ledger:l = tmp0 in
+              let hoist161:(l & Core.Option.t_Option u64) = out in
+              let ledger:l =
+                match hoist161 with
+                | Core.Option.Option_None  -> ledger
+                | Core.Option.Option_Some block_height ->
+                  Mini_ledger.LedgerData.on_purged_transaction ledger block_height
+              in
+              let ledger:l = Mini_ledger.LedgerData.pop_front_transactions_by_height ledger in
+              break_loop, ledger, num_tx_purged_out
+            | _ -> break_loop, ledger, num_tx_purged_out
+          else break_loop, ledger, num_tx_purged_out)
+  in
+  let output:usize = num_tx_purged_out in
+  ledger, output
+
+let select_accounts_to_trim
+      (#l: Type)
+      (#[FStar.Tactics.Typeclasses.tcresolve ()] __0: Core.Marker.t_Sized l)
+      (#[FStar.Tactics.Typeclasses.tcresolve ()] __1: t_LedgerData l)
+      (ledger: l)
+    : Alloc.Vec.t_Vec (Mini_ledger_core.Tokens.t_Tokens & _) Alloc.Alloc.t_Global =
+  let (to_trim: Alloc.Collections.Binary_heap.t_BinaryHeap (Mini_ledger_core.Tokens.t_Tokens & _)):Alloc.Collections.Binary_heap.t_BinaryHeap
+  (Mini_ledger_core.Tokens.t_Tokens & _) =
+    Alloc.Collections.Binary_heap.new_under_impl_9
+  in
+  let num_accounts:usize = Mini_ledger.LedgerData.accounts_overflow_trim_quantity ledger in
+  let to_trim:Alloc.Collections.Binary_heap.t_BinaryHeap (Mini_ledger_core.Tokens.t_Tokens & _) =
+    Core.Iter.Traits.Iterator.Iterator.fold (Core.Iter.Traits.Collect.IntoIterator.into_iter (Core.Iter.Traits.Iterator.Iterator.take
+              (Std.Collections.Hash.Map.iter_under_impl_1 (Mini_ledger.LedgerData.balances ledger
+                    <:
+                    Mini_ledger_core.Balances.t_Balances _
+                      (Std.Collections.Hash.Map.t_HashMap _
+                          Mini_ledger_core.Tokens.t_Tokens
+                          Std.Collections.Hash.Map.t_RandomState))
+                    .Mini_ledger_core.Balances.Balances.f_store
+                <:
+                Std.Collections.Hash.Map.t_Iter _ Mini_ledger_core.Tokens.t_Tokens)
+              num_accounts
+            <:
+            Core.Iter.Adapters.Take.t_Take
+            (Std.Collections.Hash.Map.t_Iter _ Mini_ledger_core.Tokens.t_Tokens))
+        <:
+        _)
+      to_trim
+      (fun to_trim (account, balance) ->
+          Alloc.Collections.Binary_heap.push_under_impl_9 to_trim
+            (balance, (Core.Clone.Clone.clone account <: _))
+          <:
+          Alloc.Collections.Binary_heap.t_BinaryHeap (Mini_ledger_core.Tokens.t_Tokens & _))
+  in
+  let to_trim:Alloc.Collections.Binary_heap.t_BinaryHeap (Mini_ledger_core.Tokens.t_Tokens & _) =
+    Core.Iter.Traits.Iterator.Iterator.fold (Core.Iter.Traits.Collect.IntoIterator.into_iter (Core.Iter.Traits.Iterator.Iterator.skip
+              (Std.Collections.Hash.Map.iter_under_impl_1 (Mini_ledger.LedgerData.balances ledger
+                    <:
+                    Mini_ledger_core.Balances.t_Balances _
+                      (Std.Collections.Hash.Map.t_HashMap _
+                          Mini_ledger_core.Tokens.t_Tokens
+                          Std.Collections.Hash.Map.t_RandomState))
+                    .Mini_ledger_core.Balances.Balances.f_store
+                <:
+                Std.Collections.Hash.Map.t_Iter _ Mini_ledger_core.Tokens.t_Tokens)
+              num_accounts
+            <:
+            Core.Iter.Adapters.Skip.t_Skip
+            (Std.Collections.Hash.Map.t_Iter _ Mini_ledger_core.Tokens.t_Tokens))
+        <:
+        _)
+      to_trim
+      (fun to_trim (account, balance) ->
+          match
+            Alloc.Collections.Binary_heap.peek_under_impl_10 to_trim
+            <:
+            Core.Option.t_Option (Mini_ledger_core.Tokens.t_Tokens & _)
+          with
+          | Core.Option.Option_Some (greatest_balance, _) ->
+            if balance <. greatest_balance <: bool
+            then
+              let to_trim:Alloc.Collections.Binary_heap.t_BinaryHeap
+              (Mini_ledger_core.Tokens.t_Tokens & _) =
+                Alloc.Collections.Binary_heap.push_under_impl_9 to_trim
+                  (balance, (Core.Clone.Clone.clone account <: _))
+              in
+              let tmp0, out:(Alloc.Collections.Binary_heap.t_BinaryHeap
+                (Mini_ledger_core.Tokens.t_Tokens & _) &
+                Core.Option.t_Option (Mini_ledger_core.Tokens.t_Tokens & _)) =
+                Alloc.Collections.Binary_heap.pop_under_impl_9 to_trim
+              in
+              let to_trim:Alloc.Collections.Binary_heap.t_BinaryHeap
+              (Mini_ledger_core.Tokens.t_Tokens & _) =
+                tmp0
+              in
+              let _:(Alloc.Collections.Binary_heap.t_BinaryHeap
+                (Mini_ledger_core.Tokens.t_Tokens & _) &
+                Core.Option.t_Option (Mini_ledger_core.Tokens.t_Tokens & _)) =
+                out
+              in
+              to_trim
+            else to_trim
+          | _ -> to_trim)
+  in
+  Alloc.Collections.Binary_heap.into_vec_under_impl_10 to_trim
+
+let throttle
+      (#l: Type)
+      (#[FStar.Tactics.Typeclasses.tcresolve ()] __0: Core.Marker.t_Sized l)
+      (#[FStar.Tactics.Typeclasses.tcresolve ()] __1: t_LedgerData l)
+      (ledger: l)
+      (now: Mini_ledger_core.Timestamp.t_TimeStamp)
+    : bool =
+  Rust_primitives.Hax.Control_flow_monad.Mexception.run (let num_in_window:usize =
+        Alloc.Collections.Vec_deque.len_under_impl_5 (Mini_ledger.LedgerData.transactions_by_height ledger
+
+            <:
+            Alloc.Collections.Vec_deque.t_VecDeque (Mini_ledger.Transaction.t_TransactionInfo _)
+              Alloc.Alloc.t_Global)
+      in
+      let* _:Prims.unit =
+        if
+          num_in_window >=.
+          ((Mini_ledger.LedgerData.max_transactions_in_window ledger <: usize) /. 2sz <: usize)
+        then
+          let max_rate:usize =
+            cast (((cast (Mini_ledger.LedgerData.max_transactions_in_window ledger <: usize) /. 2uL
+                    <:
+                    u64) /.
+                  (Core.Time.as_secs_under_impl_1 (Mini_ledger.LedgerData.transaction_window ledger
+                        <:
+                        Core.Time.t_Duration)
+                    <:
+                    u64)
+                  <:
+                  u64) +.
+                1uL)
+          in
+          if
+            ((Core.Option.unwrap_or_else_under_impl (Core.Option.map_under_impl (Alloc.Collections.Vec_deque.get_under_impl_5
+                          (Mini_ledger.LedgerData.transactions_by_height ledger
+                            <:
+                            Alloc.Collections.Vec_deque.t_VecDeque
+                              (Mini_ledger.Transaction.t_TransactionInfo _) Alloc.Alloc.t_Global)
+                          (Core.Num.saturating_sub_under_impl_11 num_in_window max_rate <: usize)
+                        <:
+                        Core.Option.t_Option (Mini_ledger.Transaction.t_TransactionInfo _))
+                      (fun tx -> tx.Mini_ledger.Transaction.TransactionInfo.f_block_timestamp)
+                    <:
+                    Core.Option.t_Option Mini_ledger_core.Timestamp.t_TimeStamp)
+                  (fun  ->
+                      Mini_ledger_core.Timestamp.from_nanos_since_unix_epoch_under_impl 0uL
+                      <:
+                      Mini_ledger_core.Timestamp.t_TimeStamp)
+                <:
+                Mini_ledger_core.Timestamp.t_TimeStamp) +.
+              (Core.Time.from_secs_under_impl_1 1uL <: Core.Time.t_Duration)
+              <:
+              Mini_ledger_core.Timestamp.t_TimeStamp) >.
+            now
+          then
+            let* hoist162:Rust_primitives.Hax.t_Never =
+              Core.Ops.Control_flow.ControlFlow.v_Break true
+            in
+            Core.Ops.Control_flow.ControlFlow_Continue (Rust_primitives.Hax.never_to_any hoist162)
+          else Core.Ops.Control_flow.ControlFlow_Continue ()
+        else Core.Ops.Control_flow.ControlFlow_Continue ()
+      in
+      Core.Ops.Control_flow.ControlFlow_Continue false)
+
+let apply_transaction
+      (#l: Type)
+      (#[FStar.Tactics.Typeclasses.tcresolve ()] __0: Core.Marker.t_Sized l)
+      (#[FStar.Tactics.Typeclasses.tcresolve ()] __1: t_LedgerData l)
+      (ledger: l)
+      (transaction: _)
+      (now: Mini_ledger_core.Timestamp.t_TimeStamp)
+    : (l &
+      Core.Result.t_Result
+        (u64 & Mini_ledger_core.Block.t_HashOf Mini_ledger_core.Block.t_EncodedBlock)
+        t_TransferError) =
+  Rust_primitives.Hax.Control_flow_monad.Mexception.run (let tmp0, out:(l & usize) =
+        purge_old_transactions ledger now
+      in
+      let ledger:l = tmp0 in
+      let num_pruned:(l & usize) = out in
+      let* _:Prims.unit =
+        if Prims.op_AmpAmp (num_pruned =. 0sz) (throttle ledger now)
+        then
+          let* hoist163:Rust_primitives.Hax.t_Never =
+            Core.Ops.Control_flow.ControlFlow.v_Break (ledger,
+                Core.Result.Result_Err TransferError_TxThrottled)
+          in
+          Core.Ops.Control_flow.ControlFlow_Continue (Rust_primitives.Hax.never_to_any hoist163)
+        else Core.Ops.Control_flow.ControlFlow_Continue ()
+      in
+      let maybe_time_and_hash:Core.Option.t_Option
+      (Mini_ledger_core.Timestamp.t_TimeStamp & Mini_ledger_core.Block.t_HashOf _) =
+        Core.Option.map_under_impl (Mini_ledger.LedgerTransaction.created_at_time transaction
+            <:
+            Core.Option.t_Option Mini_ledger_core.Timestamp.t_TimeStamp)
+          (fun created_at_time ->
+              created_at_time,
+              (Mini_ledger.LedgerTransaction.hash transaction <: Mini_ledger_core.Block.t_HashOf _))
+      in
+      let* _:Prims.unit =
+        match maybe_time_and_hash with
+        | Core.Option.Option_Some (created_at_time, tx_hash) ->
+          let* _:Prims.unit =
+            if
+              (created_at_time +.
+                (Mini_ledger.LedgerData.transaction_window ledger <: Core.Time.t_Duration)
+                <:
+                Mini_ledger_core.Timestamp.t_TimeStamp) <.
+              now
+            then
+              let* hoist164:Rust_primitives.Hax.t_Never =
+                Core.Ops.Control_flow.ControlFlow.v_Break (ledger,
+                    Core.Result.Result_Err
+                    (TransferError_TxTooOld
+                      ({
+                          Mini_ledger.TransferError.TxTooOld.f_allowed_window_nanos
+                          =
+                          cast (Core.Time.as_nanos_under_impl_1 (Mini_ledger.LedgerData.transaction_window
+                                    ledger
+                                  <:
+                                  Core.Time.t_Duration)
+                              <:
+                              u128)
+                        })))
+              in
+              Core.Ops.Control_flow.ControlFlow_Continue (Rust_primitives.Hax.never_to_any hoist164)
+            else Core.Ops.Control_flow.ControlFlow_Continue ()
+          in
+          let* _:Prims.unit =
+            if
+              created_at_time >.
+              (now +. v_PERMITTED_DRIFT <: Mini_ledger_core.Timestamp.t_TimeStamp)
+            then
+              let* hoist165:Rust_primitives.Hax.t_Never =
+                Core.Ops.Control_flow.ControlFlow.v_Break (ledger,
+                    Core.Result.Result_Err
+                    (TransferError_TxCreatedInFuture
+                      ({ Mini_ledger.TransferError.TxCreatedInFuture.f_ledger_time = now })))
+              in
+              Core.Ops.Control_flow.ControlFlow_Continue (Rust_primitives.Hax.never_to_any hoist165)
+            else Core.Ops.Control_flow.ControlFlow_Continue ()
+          in
+          (match
+              Alloc.Collections.Btree.Map.get_under_impl_20 (Mini_ledger.LedgerData.transactions_by_hash
+                    ledger
+                  <:
+                  Alloc.Collections.Btree.Map.t_BTreeMap (Mini_ledger_core.Block.t_HashOf _)
+                    u64
+                    Alloc.Alloc.t_Global)
+                tx_hash
+            with
+            | Core.Option.Option_Some block_height ->
+              let* hoist166:Rust_primitives.Hax.t_Never =
+                Core.Ops.Control_flow.ControlFlow.v_Break (ledger,
+                    Core.Result.Result_Err
+                    (TransferError_TxDuplicate
+                      ({ Mini_ledger.TransferError.TxDuplicate.f_duplicate_of = block_height })))
+              in
+              Core.Ops.Control_flow.ControlFlow_Continue (Rust_primitives.Hax.never_to_any hoist166)
+            | _ -> Core.Ops.Control_flow.ControlFlow_Continue ())
+        | _ -> Core.Ops.Control_flow.ControlFlow_Continue ()
+      in
+      let tmp0, out:(l & Core.Result.t_Result Prims.unit Mini_ledger_core.Balances.t_BalanceError) =
+        Mini_ledger.LedgerTransaction.apply transaction ledger
+      in
+      let ledger:l = tmp0 in
+      let hoist168:(l & Core.Result.t_Result Prims.unit Mini_ledger_core.Balances.t_BalanceError) =
+        out
+      in
+      let hoist169:Core.Result.t_Result Prims.unit t_TransferError =
+        Core.Result.map_err_under_impl hoist168
+          (function
+            | Mini_ledger_core.Balances.BalanceError_InsufficientFunds
+              { Mini_ledger_core.Balances.BalanceError.InsufficientFunds.f_balance = balance } ->
+              TransferError_InsufficientFunds
+              ({ Mini_ledger.TransferError.InsufficientFunds.f_balance = balance }))
+      in
+      let hoist170:Core.Ops.Control_flow.t_ControlFlow _ _ =
+        Core.Ops.Try_trait.Try.branch hoist169
+      in
+      let* _:Prims.unit =
+        match hoist170 with
+        | Core.Ops.Control_flow.ControlFlow_Break residual ->
+          let* hoist167:Rust_primitives.Hax.t_Never =
+            Core.Ops.Control_flow.ControlFlow.v_Break (ledger,
+                (Core.Ops.Try_trait.FromResidual.from_residual residual
+                  <:
+                  Core.Result.t_Result
+                    (u64 & Mini_ledger_core.Block.t_HashOf Mini_ledger_core.Block.t_EncodedBlock)
+                    t_TransferError))
+          in
+          Core.Ops.Control_flow.ControlFlow_Continue (Rust_primitives.Hax.never_to_any hoist167)
+        | Core.Ops.Control_flow.ControlFlow_Continue v_val ->
+          Core.Ops.Control_flow.ControlFlow_Continue v_val
+      in
+      Core.Ops.Control_flow.ControlFlow_Continue
+      (let block =
+          Mini_ledger_core.Block.BlockType.from_transaction (Mini_ledger.LedgerData.blockchain ledger
+
+              <:
+              t_Blockchain)
+              .Mini_ledger.Blockchain.f_last_hash
+            transaction
+            now
+        in
+        let block_timestamp:Mini_ledger_core.Timestamp.t_TimeStamp =
+          Mini_ledger_core.Block.BlockType.timestamp block
+        in
+        let tmp0, out:(l & Core.Result.t_Result u64 Alloc.String.t_String) =
+          Mini_ledger.LedgerData.blockchain_add_block ledger block
+        in
+        let ledger:l = tmp0 in
+        let hoist171:(l & Core.Result.t_Result u64 Alloc.String.t_String) = out in
+        let height:u64 = Core.Result.expect_under_impl hoist171 "failed to add block" in
+        let ledger:l =
+          match maybe_time_and_hash with
+          | Core.Option.Option_Some (_, tx_hash) ->
+            let tmp0, out:(l & Core.Option.t_Option u64) =
+              Mini_ledger.LedgerData.insert_transactions_by_hash ledger tx_hash height
+            in
+            let ledger:l = tmp0 in
+            let _:(l & Core.Option.t_Option u64) = out in
+            let ledger:l =
+              Mini_ledger.LedgerData.push_back_transactions_by_height ledger
+                ({
+                    Mini_ledger.Transaction.TransactionInfo.f_block_timestamp = block_timestamp;
+                    Mini_ledger.Transaction.TransactionInfo.f_transaction_hash = tx_hash
+                  })
+            in
+            ledger
+          | _ -> ledger
+        in
+        let to_trim:Alloc.Vec.t_Vec (Mini_ledger_core.Tokens.t_Tokens & _) Alloc.Alloc.t_Global =
+          if
+            (Std.Collections.Hash.Map.len_under_impl_1 (Mini_ledger.LedgerData.balances ledger
+                  <:
+                  Mini_ledger_core.Balances.t_Balances _
+                    (Std.Collections.Hash.Map.t_HashMap _
+                        Mini_ledger_core.Tokens.t_Tokens
+                        Std.Collections.Hash.Map.t_RandomState))
+                  .Mini_ledger_core.Balances.Balances.f_store
+              <:
+              usize) >=.
+            ((Mini_ledger.LedgerData.max_number_of_accounts ledger <: usize) +.
+              (Mini_ledger.LedgerData.accounts_overflow_trim_quantity ledger <: usize)
+              <:
+              usize)
+          then select_accounts_to_trim ledger
+          else Alloc.Vec.new_under_impl
+        in
+        let ledger:l =
+          Core.Iter.Traits.Iterator.Iterator.fold (Core.Iter.Traits.Collect.IntoIterator.into_iter to_trim
+
+              <:
+              _)
+            ledger
+            (fun ledger (balance, account) ->
+                let burn_tx =
+                  Mini_ledger.LedgerTransaction.burn account
+                    balance
+                    (Core.Option.Option_Some now)
+                    (Core.Option.Option_Some Mini_ledger.Transaction.v_TRIMMED_MEMO)
+                in
+                let tmp0, out:(l &
+                  Core.Result.t_Result Prims.unit Mini_ledger_core.Balances.t_BalanceError) =
+                  Mini_ledger.LedgerTransaction.apply burn_tx ledger
+                in
+                let ledger:l = tmp0 in
+                let hoist172:(l &
+                  Core.Result.t_Result Prims.unit Mini_ledger_core.Balances.t_BalanceError) =
+                  out
+                in
+                let _:Prims.unit =
+                  Core.Result.expect_under_impl hoist172
+                    "failed to burn funds that must have existed"
+                in
+                let parent_hash:Core.Option.t_Option
+                (Mini_ledger_core.Block.t_HashOf Mini_ledger_core.Block.t_EncodedBlock) =
+                  (Mini_ledger.LedgerData.blockchain ledger).Mini_ledger.Blockchain.f_last_hash
+                in
+                let tmp0, out:(l & Core.Result.t_Result u64 Alloc.String.t_String) =
+                  Mini_ledger.LedgerData.blockchain_add_block ledger
+                    (Mini_ledger_core.Block.BlockType.from_transaction parent_hash burn_tx now <: _)
+                in
+                let ledger:l = tmp0 in
+                let hoist173:(l & Core.Result.t_Result u64 Alloc.String.t_String) = out in
+                let _:u64 = Core.Result.unwrap_under_impl hoist173 in
+                ledger)
+        in
+        let output:Core.Result.t_Result
+          (u64 & Mini_ledger_core.Block.t_HashOf Mini_ledger_core.Block.t_EncodedBlock)
+          t_TransferError =
+          Core.Result.Result_Ok
+          (height,
+            Core.Option.unwrap_under_impl (Mini_ledger.LedgerData.blockchain ledger <: t_Blockchain)
+                .Mini_ledger.Blockchain.f_last_hash)
+        in
+        ledger, output))
+
+let mint_under_impl_3
+      (to: Mini_ledger.Account.t_Account)
+      (amount: Mini_ledger_core.Tokens.t_Tokens)
+      (created_at_time: Core.Option.t_Option Mini_ledger_core.Timestamp.t_TimeStamp)
+      (memo: Core.Option.t_Option Mini_ledger.Transaction.t_Memo)
+    : Mini_ledger.Transaction.t_Transaction =
+  {
+    Mini_ledger.Transaction.Transaction.f_operation
+    =
+    Mini_ledger.Transaction.Operation_Mint
+    ({
+        Mini_ledger.Transaction.Operation.Mint.f_to = to;
+        Mini_ledger.Transaction.Operation.Mint.f_amount
+        =
+        Mini_ledger_core.Tokens.get_e8s_under_impl amount
+      });
+    Mini_ledger.Transaction.Transaction.f_created_at_time
+    =
+    Core.Option.map_under_impl created_at_time
+      (fun t -> Mini_ledger_core.Timestamp.as_nanos_since_unix_epoch_under_impl t <: u64);
+    Mini_ledger.Transaction.Transaction.f_memo = memo
+  }
+
+let transfer_under_impl_3
+      (from to: Mini_ledger.Account.t_Account)
+      (amount fee: Mini_ledger_core.Tokens.t_Tokens)
+      (created_at_time: Core.Option.t_Option Mini_ledger_core.Timestamp.t_TimeStamp)
+      (memo: Core.Option.t_Option Mini_ledger.Transaction.t_Memo)
+    : Mini_ledger.Transaction.t_Transaction =
+  {
+    Mini_ledger.Transaction.Transaction.f_operation
+    =
+    Mini_ledger.Transaction.Operation_Transfer
+    ({
+        Mini_ledger.Transaction.Operation.Transfer.f_from = from;
+        Mini_ledger.Transaction.Operation.Transfer.f_to = to;
+        Mini_ledger.Transaction.Operation.Transfer.f_amount
+        =
+        Mini_ledger_core.Tokens.get_e8s_under_impl amount;
+        Mini_ledger.Transaction.Operation.Transfer.f_fee
+        =
+        Mini_ledger_core.Tokens.get_e8s_under_impl fee
+      });
+    Mini_ledger.Transaction.Transaction.f_created_at_time
+    =
+    Core.Option.map_under_impl created_at_time
+      (fun t -> Mini_ledger_core.Timestamp.as_nanos_since_unix_epoch_under_impl t <: u64);
+    Mini_ledger.Transaction.Transaction.f_memo = memo
+  }
+
+type t_Block = {
+  f_parent_hash:Core.Option.t_Option
+  (Mini_ledger_core.Block.t_HashOf Mini_ledger_core.Block.t_EncodedBlock);
+  f_transaction:Mini_ledger.Transaction.t_Transaction;
+  f_timestamp:u64
+}
+
+let v___4: Prims.unit = ()
+
+let v___5: Prims.unit = ()
+
+let t_TaggedBlock = Ciborium.Tag.t_Required t_Block 55799uL
+
+let impl: Mini_ledger_core.Block.t_BlockType t_Block =
+  {
+    transaction = Mini_ledger.Transaction.t_Transaction;
+    encode
+    =
+    (fun (self: t_Block) ->
+        let bytes:Alloc.Vec.t_Vec u8 Alloc.Alloc.t_Global = Alloc.Vec.new_under_impl in
+        let (value: Ciborium.Tag.t_Required t_Block 55799uL):Ciborium.Tag.t_Required t_Block 55799uL
+        =
+          Ciborium.Tag.Required self
+        in
+        let tmp0, out:(Alloc.Vec.t_Vec u8 Alloc.Alloc.t_Global &
+          Core.Result.t_Result Prims.unit (Ciborium.Ser.Error.t_Error _)) =
+          Ciborium.Ser.into_writer value bytes
+        in
+        let bytes:Alloc.Vec.t_Vec u8 Alloc.Alloc.t_Global = tmp0 in
+        let hoist174:(Alloc.Vec.t_Vec u8 Alloc.Alloc.t_Global &
+          Core.Result.t_Result Prims.unit (Ciborium.Ser.Error.t_Error _)) =
+          out
+        in
+        let _:Prims.unit = Core.Result.expect_under_impl hoist174 "bug: failed to encode a block" in
+        Mini_ledger_core.Block.from_vec_under_impl_8 bytes);
+    decode
+    =
+    (fun (encoded_block: Mini_ledger_core.Block.t_EncodedBlock) ->
+        Rust_primitives.Hax.Control_flow_monad.Mexception.run (let bytes:Alloc.Vec.t_Vec u8
+              Alloc.Alloc.t_Global =
+              Mini_ledger_core.Block.into_vec_under_impl_8 encoded_block
+            in
+            let* (tagged_block: Ciborium.Tag.t_Required t_Block 55799uL):Ciborium.Tag.t_Required
+              t_Block 55799uL =
+              match
+                Core.Ops.Try_trait.Try.branch (Core.Result.map_err_under_impl (Ciborium.De.from_reader
+                          (bytes.[ Core.Ops.Range.RangeFull ] <: slice u8)
+                        <:
+                        Core.Result.t_Result (Ciborium.Tag.t_Required t_Block 55799uL)
+                          (Ciborium.De.Error.t_Error _))
+                      (fun e ->
+                          Alloc.Fmt.format (Core.Fmt.new_v1_under_impl_2 (Rust_primitives.unsize (let
+                                      list =
+                                        ["failed to decode a block: "]
+                                      in
+                                      FStar.Pervasives.assert_norm
+                                      (Prims.eq2 (List.Tot.length list) 1);
+                                      Rust_primitives.Hax.array_of_list list)
+                                  <:
+                                  slice string)
+                                (Rust_primitives.unsize (let list =
+                                        [
+                                          Core.Fmt.Rt.new_display_under_impl_1 e
+                                          <:
+                                          Core.Fmt.Rt.t_Argument
+                                        ]
+                                      in
+                                      FStar.Pervasives.assert_norm
+                                      (Prims.eq2 (List.Tot.length list) 1);
+                                      Rust_primitives.Hax.array_of_list list)
+                                  <:
+                                  slice Core.Fmt.Rt.t_Argument)
+                              <:
+                              Core.Fmt.t_Arguments)
+                          <:
+                          Alloc.String.t_String)
+                    <:
+                    Core.Result.t_Result (Ciborium.Tag.t_Required t_Block 55799uL)
+                      Alloc.String.t_String)
+              with
+              | Core.Ops.Control_flow.ControlFlow_Break residual ->
+                let* hoist175:Rust_primitives.Hax.t_Never =
+                  Core.Ops.Control_flow.ControlFlow.v_Break (Core.Ops.Try_trait.FromResidual.from_residual
+                        residual
+                      <:
+                      Core.Result.t_Result t_Block Alloc.String.t_String)
+                in
+                Core.Ops.Control_flow.ControlFlow_Continue
+                (Rust_primitives.Hax.never_to_any hoist175)
+              | Core.Ops.Control_flow.ControlFlow_Continue v_val ->
+                Core.Ops.Control_flow.ControlFlow_Continue v_val
+            in
+            Core.Ops.Control_flow.ControlFlow_Continue
+            (Core.Result.Result_Ok tagged_block.Ciborium.Tag.Required.0)));
+    block_hash
+    =
+    (fun (encoded_block: Mini_ledger_core.Block.t_EncodedBlock) ->
+        Core.Result.unwrap_or_else_under_impl (Core.Result.map_under_impl (Mini_ledger.Hash.hash_cbor
+                  (Mini_ledger_core.Block.as_slice_under_impl_8 encoded_block <: slice u8)
+                <:
+                Core.Result.t_Result (array u8 32sz) Alloc.String.t_String)
+              Mini_ledger_core.Block.new_under_impl_2
+            <:
+            Core.Result.t_Result
+              (Mini_ledger_core.Block.t_HashOf Mini_ledger_core.Block.t_EncodedBlock)
+              Alloc.String.t_String)
+          (fun err ->
+              Rust_primitives.Hax.never_to_any (Core.Panicking.panic_fmt (Core.Fmt.new_v1_under_impl_2
+                        (Rust_primitives.unsize (let list =
+                                ["bug: encoded block "; " is not hashable cbor: "]
+                              in
+                              FStar.Pervasives.assert_norm (Prims.eq2 (List.Tot.length list) 2);
+                              Rust_primitives.Hax.array_of_list list)
+                          <:
+                          slice string)
+                        (Rust_primitives.unsize (let list =
+                                [
+                                  Core.Fmt.Rt.new_display_under_impl_1 (Hex.encode (Mini_ledger_core.Block.as_slice_under_impl_8
+                                            encoded_block
+                                          <:
+                                          slice u8)
+                                      <:
+                                      Alloc.String.t_String)
+                                  <:
+                                  Core.Fmt.Rt.t_Argument;
+                                  Core.Fmt.Rt.new_display_under_impl_1 err <: Core.Fmt.Rt.t_Argument
+                                ]
+                              in
+                              FStar.Pervasives.assert_norm (Prims.eq2 (List.Tot.length list) 2);
+                              Rust_primitives.Hax.array_of_list list)
+                          <:
+                          slice Core.Fmt.Rt.t_Argument)
+                      <:
+                      Core.Fmt.t_Arguments)
+                  <:
+                  Rust_primitives.Hax.t_Never)
+              <:
+              Mini_ledger_core.Block.t_HashOf Mini_ledger_core.Block.t_EncodedBlock));
+    parent_hash = (fun (self: t_Block) -> self.Mini_ledger.Block.f_parent_hash);
+    timestamp
+    =
+    (fun (self: t_Block) ->
+        Mini_ledger_core.Timestamp.from_nanos_since_unix_epoch_under_impl self
+            .Mini_ledger.Block.f_timestamp);
+    from_transaction
+    =
+    fun
+      (parent_hash:
+        Core.Option.t_Option (Mini_ledger_core.Block.t_HashOf Mini_ledger_core.Block.t_EncodedBlock)
+      )
+      (transaction: Mini_ledger.Transaction.t_Transaction)
+      (timestamp: Mini_ledger_core.Timestamp.t_TimeStamp)
+      ->
+      {
+        Mini_ledger.Block.f_parent_hash = parent_hash;
+        Mini_ledger.Block.f_transaction = transaction;
+        Mini_ledger.Block.f_timestamp
+        =
+        Mini_ledger_core.Timestamp.as_nanos_since_unix_epoch_under_impl timestamp
+      }
+  }
+
+let t_LedgerBalances =
+  Mini_ledger_core.Balances.t_Balances Mini_ledger.Account.t_Account
+    (Std.Collections.Hash.Map.t_HashMap Mini_ledger.Account.t_Account
+        Mini_ledger_core.Tokens.t_Tokens
+        Std.Collections.Hash.Map.t_RandomState)
+
+let v_TRANSACTION_WINDOW: Core.Time.t_Duration =
+  Core.Time.from_secs_under_impl_1 ((24uL *. 60uL <: u64) *. 60uL <: u64)
+
+let v_MAX_ACCOUNTS: usize = 28000000sz
+
+let v_ACCOUNTS_OVERFLOW_TRIM_QUANTITY: usize = 100000sz
+
+let v_MAX_TRANSACTIONS_IN_WINDOW: usize = 3000000sz
+
+let v_MAX_TRANSACTIONS_TO_PURGE: usize = 100000sz
+
+type t_InitArgs = {
+  f_minting_account:Mini_ledger.Account.t_Account;
+  f_initial_balances:Alloc.Vec.t_Vec (Mini_ledger.Account.t_Account & u64) Alloc.Alloc.t_Global;
+  f_transfer_fee:u64;
+  f_token_name:Alloc.String.t_String;
+  f_token_symbol:Alloc.String.t_String
+}
+
+let v___6: Prims.unit = ()
+
+let impl: Candid.Types.t_CandidType t_InitArgs =
+  {
+    _ty
+    =
+    (fun  ->
+        Candid.Types.Internal.Type_Record
+        (Alloc.Slice.into_vec_under_impl (Rust_primitives.unsize (Rust_primitives.Hax.box_new
+                  <:
+                  Alloc.Boxed.t_Box (array Candid.Types.Internal.t_Field 5sz) Alloc.Alloc.t_Global)
+              <:
+              Alloc.Boxed.t_Box (slice Candid.Types.Internal.t_Field) Alloc.Alloc.t_Global)));
+    id = (fun  -> Candid.Types.Internal.of_under_impl);
+    idl_serialize
+    =
+    fun (self: t_InitArgs) (v___serializer: v___s) ->
+      Rust_primitives.Hax.Control_flow_monad.Mexception.run (let* ser:_ =
+            match
+              Core.Ops.Try_trait.Try.branch (Candid.Types.Serializer.serialize_struct v___serializer
+                  <:
+                  Core.Result.t_Result _ _)
+            with
+            | Core.Ops.Control_flow.ControlFlow_Break residual ->
+              let* hoist176:Rust_primitives.Hax.t_Never =
+                Core.Ops.Control_flow.ControlFlow.v_Break (Core.Ops.Try_trait.FromResidual.from_residual
+                      residual
+                    <:
+                    Core.Result.t_Result Prims.unit _)
+              in
+              Core.Ops.Control_flow.ControlFlow_Continue (Rust_primitives.Hax.never_to_any hoist176)
+            | Core.Ops.Control_flow.ControlFlow_Continue v_val ->
+              Core.Ops.Control_flow.ControlFlow_Continue v_val
+          in
+          let tmp0, out:(_ & Core.Result.t_Result Prims.unit _) =
+            Candid.Types.Compound.serialize_element ser self.Mini_ledger.InitArgs.f_token_symbol
+          in
+          let ser = tmp0 in
+          let hoist178:(_ & Core.Result.t_Result Prims.unit _) = out in
+          let hoist179:Core.Ops.Control_flow.t_ControlFlow _ _ =
+            Core.Ops.Try_trait.Try.branch hoist178
+          in
+          let* _:Prims.unit =
+            match hoist179 with
+            | Core.Ops.Control_flow.ControlFlow_Break residual ->
+              let* hoist177:Rust_primitives.Hax.t_Never =
+                Core.Ops.Control_flow.ControlFlow.v_Break (Core.Ops.Try_trait.FromResidual.from_residual
+                      residual
+                    <:
+                    Core.Result.t_Result Prims.unit _)
+              in
+              Core.Ops.Control_flow.ControlFlow_Continue (Rust_primitives.Hax.never_to_any hoist177)
+            | Core.Ops.Control_flow.ControlFlow_Continue v_val ->
+              Core.Ops.Control_flow.ControlFlow_Continue v_val
+          in
+          let tmp0, out:(_ & Core.Result.t_Result Prims.unit _) =
+            Candid.Types.Compound.serialize_element ser self.Mini_ledger.InitArgs.f_transfer_fee
+          in
+          let ser = tmp0 in
+          let hoist181:(_ & Core.Result.t_Result Prims.unit _) = out in
+          let hoist182:Core.Ops.Control_flow.t_ControlFlow _ _ =
+            Core.Ops.Try_trait.Try.branch hoist181
+          in
+          let* _:Prims.unit =
+            match hoist182 with
+            | Core.Ops.Control_flow.ControlFlow_Break residual ->
+              let* hoist180:Rust_primitives.Hax.t_Never =
+                Core.Ops.Control_flow.ControlFlow.v_Break (Core.Ops.Try_trait.FromResidual.from_residual
+                      residual
+                    <:
+                    Core.Result.t_Result Prims.unit _)
+              in
+              Core.Ops.Control_flow.ControlFlow_Continue (Rust_primitives.Hax.never_to_any hoist180)
+            | Core.Ops.Control_flow.ControlFlow_Continue v_val ->
+              Core.Ops.Control_flow.ControlFlow_Continue v_val
+          in
+          let tmp0, out:(_ & Core.Result.t_Result Prims.unit _) =
+            Candid.Types.Compound.serialize_element ser self.Mini_ledger.InitArgs.f_minting_account
+          in
+          let ser = tmp0 in
+          let hoist184:(_ & Core.Result.t_Result Prims.unit _) = out in
+          let hoist185:Core.Ops.Control_flow.t_ControlFlow _ _ =
+            Core.Ops.Try_trait.Try.branch hoist184
+          in
+          let* _:Prims.unit =
+            match hoist185 with
+            | Core.Ops.Control_flow.ControlFlow_Break residual ->
+              let* hoist183:Rust_primitives.Hax.t_Never =
+                Core.Ops.Control_flow.ControlFlow.v_Break (Core.Ops.Try_trait.FromResidual.from_residual
+                      residual
+                    <:
+                    Core.Result.t_Result Prims.unit _)
+              in
+              Core.Ops.Control_flow.ControlFlow_Continue (Rust_primitives.Hax.never_to_any hoist183)
+            | Core.Ops.Control_flow.ControlFlow_Continue v_val ->
+              Core.Ops.Control_flow.ControlFlow_Continue v_val
+          in
+          let tmp0, out:(_ & Core.Result.t_Result Prims.unit _) =
+            Candid.Types.Compound.serialize_element ser self.Mini_ledger.InitArgs.f_initial_balances
+          in
+          let ser = tmp0 in
+          let hoist187:(_ & Core.Result.t_Result Prims.unit _) = out in
+          let hoist188:Core.Ops.Control_flow.t_ControlFlow _ _ =
+            Core.Ops.Try_trait.Try.branch hoist187
+          in
+          let* _:Prims.unit =
+            match hoist188 with
+            | Core.Ops.Control_flow.ControlFlow_Break residual ->
+              let* hoist186:Rust_primitives.Hax.t_Never =
+                Core.Ops.Control_flow.ControlFlow.v_Break (Core.Ops.Try_trait.FromResidual.from_residual
+                      residual
+                    <:
+                    Core.Result.t_Result Prims.unit _)
+              in
+              Core.Ops.Control_flow.ControlFlow_Continue (Rust_primitives.Hax.never_to_any hoist186)
+            | Core.Ops.Control_flow.ControlFlow_Continue v_val ->
+              Core.Ops.Control_flow.ControlFlow_Continue v_val
+          in
+          let tmp0, out:(_ & Core.Result.t_Result Prims.unit _) =
+            Candid.Types.Compound.serialize_element ser self.Mini_ledger.InitArgs.f_token_name
+          in
+          let ser = tmp0 in
+          let hoist190:(_ & Core.Result.t_Result Prims.unit _) = out in
+          let hoist191:Core.Ops.Control_flow.t_ControlFlow _ _ =
+            Core.Ops.Try_trait.Try.branch hoist190
+          in
+          let* _:Prims.unit =
+            match hoist191 with
+            | Core.Ops.Control_flow.ControlFlow_Break residual ->
+              let* hoist189:Rust_primitives.Hax.t_Never =
+                Core.Ops.Control_flow.ControlFlow.v_Break (Core.Ops.Try_trait.FromResidual.from_residual
+                      residual
+                    <:
+                    Core.Result.t_Result Prims.unit _)
+              in
+              Core.Ops.Control_flow.ControlFlow_Continue (Rust_primitives.Hax.never_to_any hoist189)
+            | Core.Ops.Control_flow.ControlFlow_Continue v_val ->
+              Core.Ops.Control_flow.ControlFlow_Continue v_val
+          in
+          Core.Ops.Control_flow.ControlFlow_Continue (Core.Result.Result_Ok ()))
+  }
+
+type t_Ledger = {
+  f_balances:Mini_ledger_core.Balances.t_Balances Mini_ledger.Account.t_Account
+    (Std.Collections.Hash.Map.t_HashMap Mini_ledger.Account.t_Account
+        Mini_ledger_core.Tokens.t_Tokens
+        Std.Collections.Hash.Map.t_RandomState);
+  f_blockchain:t_Blockchain;
+  f_minting_account:Mini_ledger.Account.t_Account;
+  f_transactions_by_hash:Alloc.Collections.Btree.Map.t_BTreeMap
+    (Mini_ledger_core.Block.t_HashOf Mini_ledger.Transaction.t_Transaction) u64 Alloc.Alloc.t_Global;
+  f_transactions_by_height:Alloc.Collections.Vec_deque.t_VecDeque
+    (Mini_ledger.Transaction.t_TransactionInfo Mini_ledger.Transaction.t_Transaction)
+    Alloc.Alloc.t_Global;
+  f_transfer_fee:Mini_ledger_core.Tokens.t_Tokens;
+  f_token_symbol:Alloc.String.t_String;
+  f_token_name:Alloc.String.t_String
+}
+
+let v___7: Prims.unit = ()
+
+let v___8: Prims.unit = ()
+
+let from_init_args_under_impl_5
+      ({ Mini_ledger.InitArgs.f_minting_account = minting_account ;
+            Mini_ledger.InitArgs.f_initial_balances = initial_balances ;
+            Mini_ledger.InitArgs.f_transfer_fee = transfer_fee ;
+            Mini_ledger.InitArgs.f_token_name = token_name ;
+            Mini_ledger.InitArgs.f_token_symbol = token_symbol }:
+          t_InitArgs)
+      (now: Mini_ledger_core.Timestamp.t_TimeStamp)
+    : t_Ledger =
+  let ledger:t_Ledger =
+    {
+      Mini_ledger.Ledger.f_balances = Core.Default.Default.v_default;
+      Mini_ledger.Ledger.f_transactions_by_hash = Alloc.Collections.Btree.Map.new_under_impl_18;
+      Mini_ledger.Ledger.f_transactions_by_height = Alloc.Collections.Vec_deque.new_under_impl_4;
+      Mini_ledger.Ledger.f_blockchain = Core.Default.Default.v_default;
+      Mini_ledger.Ledger.f_minting_account = minting_account;
+      Mini_ledger.Ledger.f_transfer_fee = Mini_ledger_core.Tokens.from_e8s_under_impl transfer_fee;
+      Mini_ledger.Ledger.f_token_symbol = token_symbol;
+      Mini_ledger.Ledger.f_token_name = token_name
+    }
+  in
+  let ledger:t_Ledger =
+    Core.Iter.Traits.Iterator.Iterator.fold (Core.Iter.Traits.Collect.IntoIterator.into_iter (Core.Iter.Traits.Collect.IntoIterator.into_iter
+              initial_balances
+            <:
+            _)
+        <:
+        _)
+      ledger
+      (fun ledger (account, balance) ->
+          let tmp0, out:(t_Ledger &
+            Core.Result.t_Result
+              (u64 & Mini_ledger_core.Block.t_HashOf Mini_ledger_core.Block.t_EncodedBlock)
+              t_TransferError) =
+            apply_transaction ledger
+              (mint_under_impl_3 (Core.Clone.Clone.clone account <: Mini_ledger.Account.t_Account)
+                  (Mini_ledger_core.Tokens.from_e8s_under_impl balance
+                    <:
+                    Mini_ledger_core.Tokens.t_Tokens)
+                  (Core.Option.Option_Some now)
+                  Core.Option.Option_None
+                <:
+                Mini_ledger.Transaction.t_Transaction)
+              now
+          in
+          let ledger:t_Ledger = tmp0 in
+          let hoist192:(t_Ledger &
+            Core.Result.t_Result
+              (u64 & Mini_ledger_core.Block.t_HashOf Mini_ledger_core.Block.t_EncodedBlock)
+              t_TransferError) =
+            out
+          in
+          let _:(u64 & Mini_ledger_core.Block.t_HashOf Mini_ledger_core.Block.t_EncodedBlock) =
+            Core.Result.unwrap_or_else_under_impl hoist192
+              (fun err ->
+                  Rust_primitives.Hax.never_to_any (Core.Panicking.panic_fmt (Core.Fmt.new_v1_under_impl_2
+                            (Rust_primitives.unsize (let list =
+                                    ["failed to mint "; " e8s to "; ": "]
+                                  in
+                                  FStar.Pervasives.assert_norm (Prims.eq2 (List.Tot.length list) 3);
+                                  Rust_primitives.Hax.array_of_list list)
+                              <:
+                              slice string)
+                            (Rust_primitives.unsize (let list =
+                                    [
+                                      Core.Fmt.Rt.new_display_under_impl_1 balance
+                                      <:
+                                      Core.Fmt.Rt.t_Argument;
+                                      Core.Fmt.Rt.new_display_under_impl_1 account
+                                      <:
+                                      Core.Fmt.Rt.t_Argument;
+                                      Core.Fmt.Rt.new_debug_under_impl_1 err
+                                      <:
+                                      Core.Fmt.Rt.t_Argument
+                                    ]
+                                  in
+                                  FStar.Pervasives.assert_norm (Prims.eq2 (List.Tot.length list) 3);
+                                  Rust_primitives.Hax.array_of_list list)
+                              <:
+                              slice Core.Fmt.Rt.t_Argument)
+                          <:
+                          Core.Fmt.t_Arguments)
+                      <:
+                      Rust_primitives.Hax.t_Never)
+                  <:
+                  (u64 & Mini_ledger_core.Block.t_HashOf Mini_ledger_core.Block.t_EncodedBlock))
+          in
+          ledger)
+  in
+  ledger
+
+let impl: t_LedgerData t_Ledger =
+  {
+    accountId = Mini_ledger.Account.t_Account;
+    transaction = Mini_ledger.Transaction.t_Transaction;
+    block = t_Block;
+    transaction_window = (fun (self: t_Ledger) -> v_TRANSACTION_WINDOW);
+    max_transactions_in_window = (fun (self: t_Ledger) -> v_MAX_TRANSACTIONS_IN_WINDOW);
+    max_transactions_to_purge = (fun (self: t_Ledger) -> v_MAX_TRANSACTIONS_TO_PURGE);
+    max_number_of_accounts = (fun (self: t_Ledger) -> v_MAX_ACCOUNTS);
+    accounts_overflow_trim_quantity = (fun (self: t_Ledger) -> v_ACCOUNTS_OVERFLOW_TRIM_QUANTITY);
+    token_name
+    =
+    (fun (self: t_Ledger) -> Core.Ops.Deref.Deref.deref self.Mini_ledger.Ledger.f_token_name);
+    token_symbol
+    =
+    (fun (self: t_Ledger) -> Core.Ops.Deref.Deref.deref self.Mini_ledger.Ledger.f_token_symbol);
+    balances = (fun (self: t_Ledger) -> self.Mini_ledger.Ledger.f_balances);
+    transfer_balance
+    =
+    (fun
+        (self: t_Ledger)
+        (from: Mini_ledger.Account.t_Account)
+        (to: Mini_ledger.Account.t_Account)
+        (amount: Mini_ledger_core.Tokens.t_Tokens)
+        (fee: Mini_ledger_core.Tokens.t_Tokens)
+        ->
+        let tmp0, out:(Mini_ledger_core.Balances.t_Balances Mini_ledger.Account.t_Account
+            (Std.Collections.Hash.Map.t_HashMap Mini_ledger.Account.t_Account
+                Mini_ledger_core.Tokens.t_Tokens
+                Std.Collections.Hash.Map.t_RandomState) &
+          Core.Result.t_Result Prims.unit Mini_ledger_core.Balances.t_BalanceError) =
+          Mini_ledger_core.Balances.transfer_under_impl_2 self.Mini_ledger.Ledger.f_balances
+            from
+            to
+            amount
+            fee
+        in
+        let self:t_Ledger = { self with Mini_ledger.Ledger.f_balances = tmp0 } in
+        let output:(Mini_ledger_core.Balances.t_Balances Mini_ledger.Account.t_Account
+            (Std.Collections.Hash.Map.t_HashMap Mini_ledger.Account.t_Account
+                Mini_ledger_core.Tokens.t_Tokens
+                Std.Collections.Hash.Map.t_RandomState) &
+          Core.Result.t_Result Prims.unit Mini_ledger_core.Balances.t_BalanceError) =
+          out
+        in
+        self, output);
+    mint_balance
+    =
+    (fun
+        (self: t_Ledger)
+        (to: Mini_ledger.Account.t_Account)
+        (amount: Mini_ledger_core.Tokens.t_Tokens)
+        ->
+        let tmp0, out:(Mini_ledger_core.Balances.t_Balances Mini_ledger.Account.t_Account
+            (Std.Collections.Hash.Map.t_HashMap Mini_ledger.Account.t_Account
+                Mini_ledger_core.Tokens.t_Tokens
+                Std.Collections.Hash.Map.t_RandomState) &
+          Core.Result.t_Result Prims.unit Mini_ledger_core.Balances.t_BalanceError) =
+          Mini_ledger_core.Balances.mint_under_impl_2 self.Mini_ledger.Ledger.f_balances to amount
+        in
+        let self:t_Ledger = { self with Mini_ledger.Ledger.f_balances = tmp0 } in
+        let output:(Mini_ledger_core.Balances.t_Balances Mini_ledger.Account.t_Account
+            (Std.Collections.Hash.Map.t_HashMap Mini_ledger.Account.t_Account
+                Mini_ledger_core.Tokens.t_Tokens
+                Std.Collections.Hash.Map.t_RandomState) &
+          Core.Result.t_Result Prims.unit Mini_ledger_core.Balances.t_BalanceError) =
+          out
+        in
+        self, output);
+    burn_balance
+    =
+    (fun
+        (self: t_Ledger)
+        (from: Mini_ledger.Account.t_Account)
+        (amount: Mini_ledger_core.Tokens.t_Tokens)
+        ->
+        let tmp0, out:(Mini_ledger_core.Balances.t_Balances Mini_ledger.Account.t_Account
+            (Std.Collections.Hash.Map.t_HashMap Mini_ledger.Account.t_Account
+                Mini_ledger_core.Tokens.t_Tokens
+                Std.Collections.Hash.Map.t_RandomState) &
+          Core.Result.t_Result Prims.unit Mini_ledger_core.Balances.t_BalanceError) =
+          Mini_ledger_core.Balances.burn_under_impl_2 self.Mini_ledger.Ledger.f_balances from amount
+        in
+        let self:t_Ledger = { self with Mini_ledger.Ledger.f_balances = tmp0 } in
+        let output:(Mini_ledger_core.Balances.t_Balances Mini_ledger.Account.t_Account
+            (Std.Collections.Hash.Map.t_HashMap Mini_ledger.Account.t_Account
+                Mini_ledger_core.Tokens.t_Tokens
+                Std.Collections.Hash.Map.t_RandomState) &
+          Core.Result.t_Result Prims.unit Mini_ledger_core.Balances.t_BalanceError) =
+          out
+        in
+        self, output);
+    blockchain = (fun (self: t_Ledger) -> self.Mini_ledger.Ledger.f_blockchain);
+    blockchain_add_block
+    =
+    (fun (self: t_Ledger) (block: t_Block) ->
+        let tmp0, out:(t_Blockchain & Core.Result.t_Result u64 Alloc.String.t_String) =
+          add_block_under_impl_2 self.Mini_ledger.Ledger.f_blockchain block
+        in
+        let self:t_Ledger = { self with Mini_ledger.Ledger.f_blockchain = tmp0 } in
+        let output:(t_Blockchain & Core.Result.t_Result u64 Alloc.String.t_String) = out in
+        self, output);
+    transactions_by_hash = (fun (self: t_Ledger) -> self.Mini_ledger.Ledger.f_transactions_by_hash);
+    remove_transactions_by_hash
+    =
+    (fun
+        (self: t_Ledger)
+        (key: Mini_ledger_core.Block.t_HashOf Mini_ledger.Transaction.t_Transaction)
+        ->
+        let tmp0, out:(Alloc.Collections.Btree.Map.t_BTreeMap
+            (Mini_ledger_core.Block.t_HashOf Mini_ledger.Transaction.t_Transaction)
+            u64
+            Alloc.Alloc.t_Global &
+          Core.Option.t_Option u64) =
+          Alloc.Collections.Btree.Map.remove_under_impl_20 self
+              .Mini_ledger.Ledger.f_transactions_by_hash
+            key
+        in
+        let self:t_Ledger = { self with Mini_ledger.Ledger.f_transactions_by_hash = tmp0 } in
+        let output:(Alloc.Collections.Btree.Map.t_BTreeMap
+            (Mini_ledger_core.Block.t_HashOf Mini_ledger.Transaction.t_Transaction)
+            u64
+            Alloc.Alloc.t_Global &
+          Core.Option.t_Option u64) =
+          out
+        in
+        self, output);
+    insert_transactions_by_hash
+    =
+    (fun
+        (self: t_Ledger)
+        (key: Mini_ledger_core.Block.t_HashOf Mini_ledger.Transaction.t_Transaction)
+        (value: u64)
+        ->
+        let tmp0, out:(Alloc.Collections.Btree.Map.t_BTreeMap
+            (Mini_ledger_core.Block.t_HashOf Mini_ledger.Transaction.t_Transaction)
+            u64
+            Alloc.Alloc.t_Global &
+          Core.Option.t_Option u64) =
+          Alloc.Collections.Btree.Map.insert_under_impl_20 self
+              .Mini_ledger.Ledger.f_transactions_by_hash
+            key
+            value
+        in
+        let self:t_Ledger = { self with Mini_ledger.Ledger.f_transactions_by_hash = tmp0 } in
+        let output:(Alloc.Collections.Btree.Map.t_BTreeMap
+            (Mini_ledger_core.Block.t_HashOf Mini_ledger.Transaction.t_Transaction)
+            u64
+            Alloc.Alloc.t_Global &
+          Core.Option.t_Option u64) =
+          out
+        in
+        self, output);
+    transactions_by_height
+    =
+    (fun (self: t_Ledger) -> self.Mini_ledger.Ledger.f_transactions_by_height);
+    pop_front_transactions_by_height
+    =
+    (fun (self: t_Ledger) ->
+        let tmp0, out:(Alloc.Collections.Vec_deque.t_VecDeque
+            (Mini_ledger.Transaction.t_TransactionInfo Mini_ledger.Transaction.t_Transaction)
+            Alloc.Alloc.t_Global &
+          Core.Option.t_Option
+          (Mini_ledger.Transaction.t_TransactionInfo Mini_ledger.Transaction.t_Transaction)) =
+          Alloc.Collections.Vec_deque.pop_front_under_impl_5 self
+              .Mini_ledger.Ledger.f_transactions_by_height
+        in
+        let self:t_Ledger = { self with Mini_ledger.Ledger.f_transactions_by_height = tmp0 } in
+        let _:(Alloc.Collections.Vec_deque.t_VecDeque
+            (Mini_ledger.Transaction.t_TransactionInfo Mini_ledger.Transaction.t_Transaction)
+            Alloc.Alloc.t_Global &
+          Core.Option.t_Option
+          (Mini_ledger.Transaction.t_TransactionInfo Mini_ledger.Transaction.t_Transaction)) =
+          out
+        in
+        self);
+    push_back_transactions_by_height
+    =
+    (fun
+        (self: t_Ledger)
+        (value: Mini_ledger.Transaction.t_TransactionInfo Mini_ledger.Transaction.t_Transaction)
+        ->
+        let self:t_Ledger =
+          {
+            self with
+            Mini_ledger.Ledger.f_transactions_by_height
+            =
+            Alloc.Collections.Vec_deque.push_back_under_impl_5 self
+                .Mini_ledger.Ledger.f_transactions_by_height
+              value
+          }
+        in
+        self);
+    on_purged_transaction = fun (self: t_Ledger) (v__height: u64) -> self
+  }
+
+let minting_account_under_impl_7 (self: t_Ledger) : Mini_ledger.Account.t_Account =
+  self.Mini_ledger.Ledger.f_minting_account
+
+let transfer_fee_under_impl_7 (self: t_Ledger) : Mini_ledger_core.Tokens.t_Tokens =
+  self.Mini_ledger.Ledger.f_transfer_fee
+
+let get_transactions_under_impl_7 (self: t_Ledger) (start: u64) (length: usize)
+    : Mini_ledger.Endpoints.t_GetTransactionsResponse =
+  let (local_transactions: Alloc.Vec.t_Vec Mini_ledger.Endpoints.t_Transaction Alloc.Alloc.t_Global):Alloc.Vec.t_Vec
+    Mini_ledger.Endpoints.t_Transaction Alloc.Alloc.t_Global =
+    Core.Iter.Traits.Iterator.Iterator.collect (Core.Iter.Traits.Iterator.Iterator.map (Core.Slice.iter_under_impl
+              (block_slice_under_impl_2 self.Mini_ledger.Ledger.f_blockchain
+                  ({
+                      Core.Ops.Range.Range.f_start = start;
+                      Core.Ops.Range.Range.f_end = start +. cast length <: u64
+                    })
+                <:
+                slice Mini_ledger_core.Block.t_EncodedBlock)
+            <:
+            Core.Slice.Iter.t_Iter Mini_ledger_core.Block.t_EncodedBlock)
+          (fun enc_block ->
+              Core.Convert.Into.into (Core.Result.expect_under_impl (Mini_ledger_core.Block.BlockType.decode
+                        (Core.Clone.Clone.clone enc_block <: Mini_ledger_core.Block.t_EncodedBlock)
+                      <:
+                      Core.Result.t_Result t_Block Alloc.String.t_String)
+                    "bug: failed to decode encoded block"
+                  <:
+                  t_Block)
+              <:
+              Mini_ledger.Endpoints.t_Transaction)
+        <:
+        Core.Iter.Adapters.Map.t_Map (Core.Slice.Iter.t_Iter Mini_ledger_core.Block.t_EncodedBlock)
+          (Mini_ledger_core.Block.t_EncodedBlock -> Mini_ledger.Endpoints.t_Transaction))
+  in
+  {
+    Mini_ledger.Endpoints.GetTransactionsResponse.f_first_index = Core.Convert.From.from start;
+    Mini_ledger.Endpoints.GetTransactionsResponse.f_log_length
+    =
+    Core.Convert.From.from (chain_length_under_impl_2 self.Mini_ledger.Ledger.f_blockchain <: u64);
+    Mini_ledger.Endpoints.GetTransactionsResponse.f_transactions = local_transactions
+  }
